TransitionSystems.v
@@ -1,14 +1,179 @@
+Require Import Notation.
 Require Import BinaryRelations.
+Require Import Privilege.
+Require Import Axioms.
+Require Import Tactics.Tactics.
 
-(* A transition relation over a global and local state *)
-Definition state_trans A B := relation (A * B).
+Open Scope string_scope.
 
-(* This mirrors Chlipala's definition of concurrent transitions in FRAP *)
-Inductive either_trans {G A B} (R: state_trans G A) (Q: state_trans G B)
-  : state_trans G (A * B) :=
-  | step_l : forall g g' a a' b,
-      R (g,a) (g',a') -> either_trans R Q (g,(a,b)) (g',(a',b))
-  | step_r : forall g g' a b b',
-      Q (g,b) (g',b') -> either_trans R Q (g,(a,b)) (g',(a,b')).
-    
-Notation "R ⊔ S" := (either_trans R S) (at level 70).
+(* Dynamic environments (partial maps from variables to arbitrary types) *)
+
+(* TODO: abstract as a section variable? *)
+Definition var  := string.
+Definition comp := string.
+
+Definition env := var -> option (access × Σ V, V).
+
+Declare Scope env_scope.
+(* Delimit Scope env_scope with env. *)
+Bind Scope env_scope with env.
+Open Scope env_scope.
+
+
+Definition env_empty: env := λ _, None.
+Notation "•" := env_empty : env_scope.
+
+Definition env_singleton {V} var (acc: access) (v: V): env := λ lookup,
+  if lookup =? var then Some (acc, existT _ V v) else None.
+Notation "var ↦ v" := (env_singleton var allAcc v)
+  (at level 55, right associativity) : env_scope.
+
+Definition map_access (Γ: env) (acc: access): env := λ lookup, 
+  match Γ lookup with 
+  | Some (_, v) => Some (acc, v)
+  | None => None
+  end.
+Notation "acc ? Γ" := (map_access Γ acc)
+  (at level 60) : env_scope.
+  (* (at level 60, format "acc ?  Γ") : env_scope. *)
+
+(* First env shadows definitions in second *)
+Definition env_concat (Γ1 Γ2: env) : env := λ lookup,
+  match Γ1 lookup with 
+  | Some v => Some v 
+  | None => Γ2 lookup
+  end.
+Notation "Γ1 ;; Γ2" := (env_concat Γ1 Γ2)
+  (at level 65, right associativity) : env_scope.
+
+Definition read {V} (Γ: env) (c: comp) (name: var) (v: V) : Prop :=
+  exists! acc: access, 
+    Γ name = Some (acc, existT _ V v) /\
+    acc c p_read.
+
+Definition write {V} (Γ: env) (c: comp) (name: var) (v: V) (Γ': env) : Prop :=
+  exists! (acc: access) curr,
+    Γ name = Some (acc, curr) /\ 
+    acc c p_write /\ 
+    Γ' = acc ? name ↦ v ;; Γ.
+
+Definition remove_var (Γ: env) var : env := λ lookup,
+  if lookup =? var then None else Γ lookup.
+
+Lemma map_acc_env_singleton : forall acc x V (v: V),
+  (acc ? x ↦ v) = env_singleton x acc v.
+Proof using.
+  intros *.
+  extensionality y.
+  unfold env_singleton.
+  replace (
+    acc ? (λ lookup, 
+      if lookup =? x
+      then Some (allAcc, existT _ V v) 
+      else None))
+  with
+    (λ lookup, 
+      if lookup =? x
+      then Some (acc, existT _ V v) 
+      else None
+  ).
+  - reflexivity.
+  - extensionality lookup.
+    unfold map_access.
+    now destruct (lookup =? x).
+Qed.
+
+Lemma refl_string_eq : forall x y,
+  x =? y ->
+  x = y.
+Proof using.
+  intros * ?.
+  now destruct (eqb_spec x y).
+Qed.
+
+Theorem env_singleton_inv : forall acc x y V (v: V) v',
+  (acc ? x ↦ v) y = Some v' ->
+  x = y /\ v' = (acc, existT _ V v).
+Proof using.
+  intros * H.
+  rewrite map_acc_env_singleton in H.
+  unfold env_singleton in H.
+  destruct (y =? x) eqn:case; [|discriminate].
+  apply refl_string_eq in case as ->.
+  now inv H.
+Qed.
+
+Theorem env_prepend_singleton_unchanged : forall (Γ: env) x y acc V (v: V),
+  x <> y ->
+  Γ y = (acc ? x ↦ v ;; Γ) y.
+Proof using.
+  intros * Hneq.
+  unfold env_concat.
+  destruct ((acc ? x ↦ v) y) eqn:case. 
+  - apply env_singleton_inv in case as [-> _].
+    contradiction.
+  - reflexivity.
+Qed.
+
+Theorem write_unchanged : forall Γ Γ' x y c V (v: V),
+  write Γ c x v Γ' ->
+  x <> y ->
+  Γ y = Γ' y.
+Proof using.
+  intros * Hwrite Hneq.
+  destruct Hwrite as [acc [[curr [(Hwrite1 & Hwrite2 & ->) _]] _]].
+  now apply env_prepend_singleton_unchanged.
+Qed.
+
+Theorem write_unchanged_read : forall Γ Γ' x y c c' V (v: V) V' (v': V'),
+  write Γ c x v Γ' ->
+  x <> y ->
+  read Γ c' y v' ->
+  read Γ' c' y v'.
+Proof using. 
+  intros * Hwrite Hneq Hread.
+  unfold read in *.
+  destruct Hread as (acc & (Hlookup & Hacc) & Hunique).
+  exists acc.
+  max split.
+  - rewrite <- Hlookup.
+    symmetry.
+    enow eapply write_unchanged.
+  - assumption.
+  - intros * [H _].
+    erewrite <- write_unchanged in H; [|eassumption|eassumption].
+    rewrite Hlookup in H.
+    now inv H.
+Qed.
+
+Theorem write_unchanged_read' : forall Γ Γ' x y c c' V (v: V) V' (v': V'),
+  write Γ c x v Γ' ->
+  x <> y ->
+  read Γ' c' y v' ->
+  read Γ c' y v'.
+Proof using. 
+  intros * Hwrite Hneq Hread.
+  unfold read in *.
+  destruct Hread as (acc & (Hlookup & Hacc) & Hunique).
+  exists acc.
+  max split.
+  - rewrite <- Hlookup.
+    enow eapply write_unchanged.
+  - assumption.
+  - intros * [H _].
+    erewrite <- write_unchanged in Hlookup; [|eassumption|eassumption].
+    rewrite Hlookup in H.
+    now inv H.
+Qed.
+
+Theorem no_lookup_no_read : forall Γ c x V (v: V),
+  Γ x = None -> ~ read Γ c x v.
+Proof using.
+  intros * Heq Hread.
+  destruct Hread as (acc & (Heq' & _) & _).
+  rewrite Heq in Heq'.
+  discriminate Heq'.
+Qed.
+
+Close Scope env_scope.
+Close Scope string_scope.
