Notation.v
@@ -3,17 +3,42 @@ Require Import Coq.Logic.JMeq.
 
 Notation "x ~= y" := (JMeq x y) (at level 70, no associativity).
 
+
 Notation "'sigma' x .. y , p" := (sigT (fun x => .. (sigT (fun y => p)) ..))
-  (at level 200, x binder, right associativity,
-   format "'[' 'sigma' '/ ' x .. y , '/  ' p ']'")
+  (at level 200, x binder, y binder, right associativity,
+   only parsing)
   : type_scope.
+   (* format "'[' 'sigma' '/ ' x .. y , '/  ' p ']'") *)
 
 Notation "'Σ' x .. y , p" := (sigT (fun x => .. (sigT (fun y => p)) ..))
-  (at level 200, x binder, right associativity,
+  (at level 200, x binder, y binder, right associativity,
    format "'[' 'Σ'  '/ ' x .. y , '/ '  p ']'")
   : type_scope.
 
 
+Notation "x × y" := (prod x y) (at level 40, left associativity): type_scope.
+
+
+Notation "'Π'  x .. y , P" := (forall x, .. (forall y, P) ..)
+  (at level 200, x binder, y binder, right associativity,
+   only parsing)
+  : type_scope.
+   (* format "'[' 'Π'  '/ ' x .. y , '/ '  P ']'") *)
+
+Notation "'∀'  x .. y , P" := (forall x, .. (forall y, P) ..)
+  (at level 200, x binder, y binder, right associativity,
+   format "'[' '∀'  '/ ' x .. y , '/ '  P ']'")
+  : type_scope.
+
+
 Notation "'λ' x .. y , b" := (fun x => .. (fun y => b) ..)
-  (at level 200, x binder, right associativity,
+  (at level 200, x binder, y binder, right associativity,
    format "'[' 'λ' '/ ' x .. y , '/ '  b ']'").
+
+
+Definition is_true (b: bool) := b = true.
+Coercion is_true : bool >-> Sortclass.
+
+(* Notation "'𝔹'" := bool.
+Notation "'ℕ'" := nat.
+Notation "'ℙ'" := Prop. *)
